coq_translation/examples/conversion/try_from_and_try_into.v
@@ -36,7 +36,7 @@ Module
   Definition Self := try_from_and_try_into.EvenNumber.
   
   Global Instance I : core.marker.StructuralPartialEq.Trait Self :=
-    core.marker.StructuralPartialEq.Build_Class _.
+    core.marker.StructuralPartialEq.Build_Trait _.
 End Impl_core_marker_StructuralPartialEq_for_try_from_and_try_into_EvenNumber.
 
 Module Impl_core_cmp_PartialEq_for_try_from_and_try_into_EvenNumber.
