coq_translation/examples/generics/generics_bounds_test_case_empty_bounds.v
@@ -18,14 +18,14 @@ Definition Turkey := Turkey.t.
 
 Module Red.
   Unset Primitive Projections.
-  Class Trait (Self : Set) : Set := {
+  Class Trait (Self : Set) : Set := {  
   }.
   Global Set Primitive Projections.
 End Red.
 
 Module Blue.
   Unset Primitive Projections.
-  Class Trait (Self : Set) : Set := {
+  Class Trait (Self : Set) : Set := {  
   }.
   Global Set Primitive Projections.
 End Blue.
@@ -35,7 +35,7 @@ Module
   Definition Self := generics_bounds_test_case_empty_bounds.Cardinal.
   
   Global Instance I : generics_bounds_test_case_empty_bounds.Red.Trait Self :=
-    generics_bounds_test_case_empty_bounds.Red.Build_Class _.
+    generics_bounds_test_case_empty_bounds.Red.Build_Trait _.
 End
   Impl_generics_bounds_test_case_empty_bounds_Red_for_generics_bounds_test_case_empty_bounds_Cardinal.
 
@@ -44,7 +44,7 @@ Module
   Definition Self := generics_bounds_test_case_empty_bounds.BlueJay.
   
   Global Instance I : generics_bounds_test_case_empty_bounds.Blue.Trait Self :=
-    generics_bounds_test_case_empty_bounds.Blue.Build_Class _.
+    generics_bounds_test_case_empty_bounds.Blue.Build_Trait _.
 End
   Impl_generics_bounds_test_case_empty_bounds_Blue_for_generics_bounds_test_case_empty_bounds_BlueJay.
 
