coq_translation/examples/traits/clone.v
@@ -42,7 +42,7 @@ Module Impl_core_marker_Copy_for_clone_Unit.
   Definition Self := clone.Unit.
   
   Global Instance I : core.marker.Copy.Trait Self :=
-    core.marker.Copy.Build_Class _.
+    core.marker.Copy.Build_Trait _.
 End Impl_core_marker_Copy_for_clone_Unit.
 
 Module Pair.
