coq_translation/examples/traits/disambiguating_overlapping_traits.v
@@ -2,7 +2,7 @@
 Require Import CoqOfRust.CoqOfRust.
 
 Module UsernameWidget.
-  Class Trait (Self : Set) : Set := {
+  Class Trait (Self : Set) : Set := {  
     get : (ref Self) -> (M alloc.string.String);
   }.
   
@@ -12,7 +12,7 @@ Module UsernameWidget.
 End UsernameWidget.
 
 Module AgeWidget.
-  Class Trait (Self : Set) : Set := {
+  Class Trait (Self : Set) : Set := {  
     get : (ref Self) -> (M u8);
   }.
   
